Finish proof of SHA3 is incremental

specs/lemmas/Spec.SHA3.Incremental.fst
@@ -167,36 +167,6 @@ let sha3_is_incremental1
      );
   }
 
-(*
-let sha3_update (a: sha3_alg) (s: words_state' a) (b: bytes { S.length b = block_length a }): words_state' a =
-    let rateInBytes = 1088 / 8 in
-  Spec.SHA3.absorb_inner rateInBytes b s
-
-let sha3_update_last (a: sha3_alg) (s: words_state' a) (l: bytes { S.length l < block_length a }):
-  words_state' a
-=
-  let rateInBytes = 1088 / 8 in
-  let delimitedSuffix = byte 0x06 in
-  Spec.SHA3.absorb_last delimitedSuffix rateInBytes (S.length l) l s
-
-#push-options "--fuel 1"
-let rec sha3_ignores_extra_state (a: sha3_alg) (acc: words_state' a) (bs: bytes): Lemma
-  (requires S.length bs % block_length a = 0)
-  (ensures (
-    let acc1, () = Lib.UpdateMulti.mk_update_multi (block_length a) (update a) (acc, ()) bs in
-    let acc2 = Lib.UpdateMulti.mk_update_multi (block_length a) (sha3_update a) acc bs in
-    acc1 == acc2))
-  (decreases S.length bs)
-=
-  if S.length bs = 0 then
-    ()
-  else
-    let block, rem = Lib.UpdateMulti.split_block (block_length a) bs 1 in
-    let acc = sha3_update a acc block in
-    sha3_ignores_extra_state a acc rem
-#pop-options
-*)
-
 let sha3_is_incremental2
   (a: sha3_alg)
   (input: bytes): Lemma (hash a input `S.equal` (
@@ -207,121 +177,38 @@ let sha3_is_incremental2
     let s = update_multi a s () bs in
     let s = Spec.SHA3.absorb_last delimitedSuffix rateInBytes (S.length l) l s in
     finish a s))
-= admit()
+= let rateInBytes = 1088 / 8 in
+  let delimitedSuffix = byte 0x06 in
+  let nb = S.length input / block_length a in
+  let s = Lib.Sequence.create 25 (u64 0) in
+  let bs, l = UpdateMulti.split_at_last rateInBytes input in
+  assert (S.length bs / block_length a == nb);
+  let f = Spec.SHA3.absorb_inner rateInBytes in
+  calc (==) {
+    hash a input;
+    (==) { } (
+      let s = Spec.SHA3.absorb s rateInBytes (S.length input) input delimitedSuffix in
+      Spec.SHA3.squeeze s rateInBytes 32
+      );
+   (==) { Lib.Sequence.lemma_repeat_blocks (block_length a) input f (Spec.SHA3.absorb_last delimitedSuffix rateInBytes) s } (
+      let s = Loops.repeati #(words_state a) nb (Lib.Sequence.repeat_blocks_f (block_length a) input f nb) s in
+      let s = Spec.SHA3.absorb_last delimitedSuffix rateInBytes (S.length l) l s in
+      Spec.SHA3.squeeze s rateInBytes 32);
+   (==) {
+     Lib.Sequence.Lemmas.repeati_extensionality #(words_state a) nb
+       (Lib.Sequence.repeat_blocks_f (block_length a) input f nb)
+       (Lib.Sequence.repeat_blocks_f (block_length a) bs f nb)
+       s
+     } (
+      let s = Loops.repeati #(words_state a) nb (Lib.Sequence.repeat_blocks_f (block_length a) bs f nb) s in
+      let s = Spec.SHA3.absorb_last delimitedSuffix rateInBytes (S.length l) l s in
+      Spec.SHA3.squeeze s rateInBytes 32);
+   (==) { Lib.Sequence.lemma_repeat_blocks_multi #_ #(words_state a) (block_length a) bs f s } (
+      let s = Lib.Sequence.repeat_blocks_multi #_ #(words_state a) (block_length a) bs f s in
+      let s = Spec.SHA3.absorb_last delimitedSuffix rateInBytes (S.length l) l s in
+      Spec.SHA3.squeeze s rateInBytes 32);
+    }
 
-(*
-  calc (S.equal) { (
-    let s = Lib.Sequence.create 25 (u64 0), () in
-    let rateInBytes = 1088 / 8 in
-    let delimitedSuffix = byte 0x06 in
-    let bs, l = UpdateMulti.split_at_last rateInBytes input in
-    let s, _ = update_multi a s bs in
-    let s = Spec.SHA3.absorb_last delimitedSuffix rateInBytes (S.length l) l s, () in
-    finish a s
-  );
-  (S.equal) {
-  } (
-    let s = Lib.Sequence.create 25 (u64 0), () in
-    let rateInBytes = 1088 / 8 in
-    let delimitedSuffix = byte 0x06 in
-    let bs, l = UpdateMulti.split_at_last rateInBytes input in
-    let s, _ = Lib.UpdateMulti.mk_update_multi (block_length a) (update a) s bs in
-    let s = Spec.SHA3.absorb_last delimitedSuffix rateInBytes (S.length l) l s, () in
-    finish a s
-  );
-  (S.equal) {
-    let s = Lib.Sequence.create 25 (u64 0) in
-    let rateInBytes = 1088 / 8 in
-    let delimitedSuffix = byte 0x06 in
-    let bs, l = UpdateMulti.split_at_last rateInBytes input in
-    sha3_ignores_extra_state a s bs
-  } (
-    let s = Lib.Sequence.create 25 (u64 0) in
-    let rateInBytes = 1088 / 8 in
-    let delimitedSuffix = byte 0x06 in
-    let bs, l = UpdateMulti.split_at_last rateInBytes input in
-    let s, () = Lib.UpdateMulti.mk_update_multi #(words_state' a) (block_length a) (sha3_update a) s bs, () in
-    let s = Spec.SHA3.absorb_last delimitedSuffix rateInBytes (S.length l) l s, () in
-    finish a s
-  );
-  // This step does not work unless the type argument to update_multi is
-  // explicitly instantiated. The trefl is here only to help debug. Use
-  // #set-options "--print_implicits" to see the issue.
-  (==) {
-    (_ by (FStar.Tactics.trefl()))
-  } (
-    let s = Lib.Sequence.create 25 (u64 0) in
-    let rateInBytes = 1088 / 8 in
-    let delimitedSuffix = byte 0x06 in
-    let bs, l = UpdateMulti.split_at_last rateInBytes input in
-    let s = Lib.UpdateMulti.mk_update_multi #(words_state' a) (block_length a) (sha3_update a) s bs in
-    let s = Spec.SHA3.absorb_last delimitedSuffix rateInBytes (S.length l) l s, () in
-    finish a s
-  );
-  (S.equal) {
-  } (
-    let s = Lib.Sequence.create 25 (u64 0) in
-    let rateInBytes = 1088 / 8 in
-    let delimitedSuffix = byte 0x06 in
-    let bs, l = UpdateMulti.split_at_last rateInBytes input in
-    let s = Lib.UpdateMulti.mk_update_multi #(words_state' a) (block_length a) (sha3_update a) s bs in
-    let s = sha3_update_last a s l, () in
-    finish a s
-  );
-  (==) {
-    let s = Lib.Sequence.create 25 (u64 0) in
-    let rateInBytes = 1088 / 8 in
-    Lib.UpdateMulti.Lemmas.update_full_is_repeat_blocks rateInBytes (sha3_update a) (sha3_update_last a) s input input
-  } (
-    let s = Lib.Sequence.create 25 (u64 0) in
-    let rateInBytes = 1088 / 8 in
-    let delimitedSuffix = byte 0x06 in
-    let s = Lib.Sequence.repeat_blocks #uint8 rateInBytes input
-      (Lib.UpdateMulti.Lemmas.repeat_f rateInBytes (sha3_update a))
-      (Lib.UpdateMulti.Lemmas.repeat_l rateInBytes (sha3_update_last a) input)
-      s, ()
-    in
-    finish a s
-  );
-  (==) {
-    let s = Lib.Sequence.create 25 (u64 0) in
-    let rateInBytes = 1088 / 8 in
-    let delimitedSuffix = byte 0x06 in
-    Lib.Sequence.Lemmas.repeat_blocks_extensionality #uint8 #(words_state' a) #(words_state' a) rateInBytes input
-      (Lib.UpdateMulti.Lemmas.repeat_f rateInBytes (sha3_update a))
-      (Spec.SHA3.absorb_inner rateInBytes)
-      (Lib.UpdateMulti.Lemmas.repeat_l rateInBytes (sha3_update_last a) input)
-      (Spec.SHA3.absorb_last delimitedSuffix rateInBytes)
-      s
-  } (
-    let s = Lib.Sequence.create 25 (u64 0) in
-    let rateInBytes = 1088 / 8 in
-    let delimitedSuffix = byte 0x06 in
-    let s = Lib.Sequence.repeat_blocks #uint8 #(words_state' a) #(words_state' a) rateInBytes input
-      (Spec.SHA3.absorb_inner rateInBytes)
-      (Spec.SHA3.absorb_last delimitedSuffix rateInBytes)
-      s, ()
-    in
-    finish a s
-  );
-  (==) {
-    // sha3_state_is_hash_state
-  } (
-    let s = Lib.Sequence.create 25 (u64 0) in
-    let rateInBytes = 1088 / 8 in
-    let delimitedSuffix = byte 0x06 in
-    let s = Lib.Sequence.repeat_blocks #uint8 #Spec.SHA3.state #Spec.SHA3.state rateInBytes input
-      (Spec.SHA3.absorb_inner rateInBytes)
-      (Spec.SHA3.absorb_last delimitedSuffix rateInBytes)
-      s
-    in
-    Spec.SHA3.squeeze s rateInBytes 32
-  );
-  (==) {
-  }
-    Spec.SHA3.sha3_256 (S.length input) input;
-  }
-*)
 let sha3_is_incremental
   (a: sha3_alg)
   (input: bytes): Lemma (hash_incremental a input `S.equal` hash a input)
